fr.inria.atlanmod.coqtl.coq/examples/Graph2Tree/GraphTest.v
@@ -1,0 +1,68 @@
+Require Import String.
+Require Import List.
+
+Require Import core.CoqTL.
+Require Import core.utils.tPrint.
+Require Import core.Model.
+
+Require Import examples.ClassGraph2Tree.ClassMetamodel.
+Require Import examples.ClassGraph2Tree.ClassGraph2Tree.
+Require Import examples.ClassGraph2Tree.PersonModel.
+Require Import core.utils.tTop.
+Compute execute ClassGraph2Tree PersonModel. 
+ 
+
+
+(* Definition getFors  (tr: TransformationA ClassMetamodel ClassMetamodel)  : ForExpressionA :=
+match (TransformationA_getRules tr) with
+|  r :: _ => (RuleA_getForExpression r)
+| _ => BuildForExpressionA 999
+end.
+
+
+Definition sp := (Build_ClassMetamodel_EObject ClassEClass (BuildClass "0" "Person")) :: nil.
+Definition sm := PersonModel.
+Definition tr := ClassGraph2Tree.
+
+(* Compute (
+fets <- (evalForExpression (getFors tr) tr sm sp);
+path <- nth_error  fets 1 ;
+path_id <- index path (allPathsTo sm 1 (BuildClass "0" "Person")); 
+cls <- resolveIter tr sm "cl" ClassEClass sp path_id;
+Some cls
+). *)
+
+
+
+Compute (
+match matchPattern tr sm sp with
+    | nil => None
+    | l => Some (map 
+(fun r => 
+
+let outs := (RuleA_getOutputPattern r) in
+ out <- nth_error outs 2;
+Some (beq_string (OutputPatternElementA_getName out) "cl")
+
+
+
+(* return optionList2List (flat_map (fun te => flat_map (fun bind => (map (fun fe => applyOutputPatternReferencesOnPatternIter r tr sm sp fe bind te) fets)) binds) tes)
+  *)
+
+
+)
+                l) 
+end).
+
+Compute 
+( let f := (getFors ClassGraph2Tree) in
+  ope <- (find_OutputPatternElementA tr sm sp "cl");
+  r <- Some (OutputPatternElementExpressionA_getRule (OutputPatternElementA_getOutputPatternElementExpression ope));
+  ra <- (nth_error (TransformationA_getRules tr) r);
+  fe_res <- (evalForExpression f tr sm sp);
+  fet <- nth_error fe_res 0;
+  let  opee := (OutputPatternElementA_getOutputPatternElementExpression ope) in 
+   tfe <- ForExpressionA_getForSectionType2OutputPatternElementExpressionA f opee tr sp sm fet;
+  (evalOutputPatternElementExpressionWithIter (OutputPatternElementA_getOutputPatternElementExpression ope) tr sm sp tfe)
+
+  ).   *)
